theories/L6_PCPS/hoisting.v
@@ -1,35 +1,62 @@
-Require Import cps cps_util shrink_cps identifiers.
-Require Import BinNat Relations.
+Require Import cps cps_util shrink_cps identifiers eval env ctx.
+Require Import List BinNat Relations.
+
+Import ListNotations.
 
 (* TODO : move dependencies from shrink_cps to common file *)
 
-Fixpoint exp_hoist (e : exp) (defs : fundefs ) (f : exp -> exp) : exp :=
+Fixpoint exp_hoist (e : exp) (defs : fundefs)
+         (f : exp * fundefs -> exp * fundefs) {struct e} : exp * fundefs :=
   match e with
     | Econstr x typ tag ys e' =>
-      exp_hoist e' defs (fun e => f (Econstr x typ tag ys e))
-    | Ecase x xs =>
-      Efun defs (f (Ecase x xs))
+      exp_hoist e' defs (fun p => let (e, defs) := p in
+                                  f (Econstr x typ tag ys e, defs))
+    | Ecase x tes =>
+      fold_left
+        (fun (f : exp * fundefs -> exp * fundefs) (te : tag * exp) =>
+           fun p =>
+             let (c, e) := te in
+             let (e1, defs1) := p in
+             exp_hoist e defs1
+                       (fun p2 =>
+                          let (e2, defs2) := p2 in
+                          match e1 with
+                            | Ecase x' tes' =>
+                              f (Ecase x' ((c, e2) :: tes), defs2)
+                            | _ => (* This should never match *)
+                              f (Ecase x [(c, e2)], defs2)
+                          end)) tes f (Ecase x tes, defs)
     | Eproj x typ n y e' =>
-      exp_hoist e' defs (fun e => f (Eproj x typ n y e))
-    | Efun fdefs e =>
-      let defs' := fundefs_hoist fdefs defs id in
-      exp_hoist e defs' f 
+      exp_hoist e' defs (fun p =>
+                           let (e, defs) := p in
+                           f (Eproj x typ n y e, defs))
+    | Efun fdefs e' =>
+      exp_hoist e' defs (fun p =>
+                           let (e'', defs'') := p in
+                           fundefs_hoist fdefs e'' defs'' f)
     | Eapp g xs =>
-      Efun defs (f (Eapp g xs))
+      f (Eapp g xs, defs)
     | Eprim x typ prim ys e' =>
-      exp_hoist e' defs (fun e => f (Eprim x typ prim ys e))
+      exp_hoist e' defs (fun p =>
+                           let (e', defs') := p in
+                           f (Eprim x typ prim ys e', defs'))
   end
-with fundefs_hoist (defs hdefs : fundefs) (f : fundefs -> fundefs) :
-       fundefs :=
-  match defs with 
-    | Fcons g t xs e defs =>
-      match exp_hoist e hdefs id with
-        | Efun hdefs' e' =>
-          fundefs_hoist defs hdefs' (fun d => f (Fcons g t xs e' d)) 
-        | _ => hdefs
-      end
-    | Fnil => f hdefs 
+with fundefs_hoist (defs : fundefs) (e : exp) (hdefs : fundefs)
+                   (f : exp * fundefs -> exp * fundefs) {struct defs}
+     : exp * fundefs :=
+       match defs with 
+         | Fcons g t xs e defs =>
+           fundefs_hoist defs e hdefs
+                         (fun p1 =>
+                            let (e1, defs1) := p1 in
+                            exp_hoist e defs1
+                                      (fun p2 =>
+                                         let (e2, defs2) := p1 in
+                                         (e1, Fcons g t xs e2 defs2)))
+         | Fnil => f (e, hdefs)
   end.
+
+
 
 (** expressions without function definitions *)
 Inductive no_fun : exp -> Prop  :=
@@ -111,6 +138,8 @@ Proof.
   unfold injective; eauto.
 Qed.
 
+(* The following need to be updated.
+
 Lemma exp_fundefs_hoist_no_fun:
   (forall e,
    exists g e',
@@ -126,12 +155,12 @@ Lemma exp_fundefs_hoist_no_fun:
      injective g /\
      forall defs, no_fun_defs defs -> no_fun_defs (g defs)).
 Proof.
-  exp_defs_induction IHe IHf;
+  exp_defs_induction IHe IHl IHf;
   intros; try edestruct IHe as [g1 [? [H1 [H2 [H3 H4]]]]];
   try edestruct IHf as [g2 [H5 [H6 H7]]];
   try (now do 2 eexists; 
        simpl; split; [ intros defs f; rewrite H1; eauto | split; eauto ]);
-  try (now exists id; repeat eexists; intros; unfold injective; eauto). 
+  try (now exists id; repeat eexists; intros; unfold injective; eauto).
   simpl. exists (fun x => g1 (g2 x)); eexists.
   split; intros. rewrite H1, H5; eauto.
   split; eauto using injective_comp.
@@ -173,16 +202,6 @@ Proof.
 Qed.
 
 
-Lemma app_ctx_fuse:
-  forall (c c' : exp_ctx) (e1 e2 e3 : exp),
-    app_ctx c e1 e2 ->
-    app_ctx c' e2 e3 ->
-    app_ctx (comp_ctx_f c' c) e1 e3.
-Proof.
-  intros c c' e1 e2 e3 H1 H2. rewrite <- app_ctx_f_correct.
-  rewrite <- app_ctx_f_fuse.
-  rewrite <- app_ctx_f_correct in H1, H2. rewrite H1. eauto.
-Qed.
 
 Lemma hoist_star_0 :
   forall e e', hoist_star_n 0 e e' -> e = e'.
@@ -261,7 +280,8 @@ Lemma exp_fundefs_hoist_in_hoist_star :
                 (Efun (fundefs_hoist defs hdefs f) (g e))).
 Proof.
   apply exp_def_mutual_ind;
-  [intros x typ tag ys e IHe  fdefs f Hctx | intros x t_ys  fdefs f Hctx
+  [intros x typ tag ys e IHe  fdefs f Hctx | intros x fdefs f Hctx
+   | intros x tes c e IHe IHl fdefs f Hctx
    | intros x typ n y e IHe fdefs f Hctx | intros defs IHdefs e IHe fdefs f Hctx
    | intros g xs fdefs f Hctx
    | intros x  typ pr ys e IHe fdefs f Hctx
@@ -274,7 +294,9 @@ Proof.
     eexists (comp_ctx_f c (Econstr_c x typ tag ys Hole_c)).
     intros e'. rewrite <- Hctx. now rewrite <- app_ctx_f_fuse. 
   - eexists. apply hoistn_refl.
-  - simpl. specialize (IHe fdefs (fun e => f (Eproj x typ n y e))).
+  -  
+
+    - simpl. specialize (IHe fdefs (fun e => f (Eproj x typ n y e))).
     apply IHe.
     destruct Hctx as [c Hctx].
     eexists (comp_ctx_f c (Eproj_c x typ n y Hole_c)).
@@ -311,12 +333,133 @@ Proof.
     apply app_ctx_f_correct. simpl. f_equal; eauto.
 Qed.
 
+Open Scope ctx_scope.
+Open Scope env_scope.
 
-Lemma hoist_rw_correct (pr : prims) (e1 e2 : exp) (rho : env) (obs : obs_val) :
-  closed_fundefs_in_exp e1 ->
-  unique_bindings e1 ->
-  hoist_rw e1 e2 ->
-  bstep_e pr rho e1 obs ->
-  bstep_e pr rho e2 obs.
+Lemma preord_env_permut k x y v1 v2 rho1 rho2 :
+  x <> y ->
+  preord_env k (M.set x v1 (M.set y v2 rho1)) (M.set x v1 (M.set y v2 rho2)) ->
+  preord_env k (M.set x v1 (M.set y v2 rho1)) (M.set y v2 (M.set x v1 rho2)).
 Proof.
-Abort.
+  intros Hneq Hpre x' v1' Hget.
+  rewrite M.gsspec in Hget.
+  destruct (Coqlib.peq x' x). inv Hget. 
+  - edestruct (Hpre x) as [v1'' [Hget'' Hpre'']]. rewrite M.gss; eauto.
+    rewrite M.gss in Hget''; inv Hget''.
+    eexists. rewrite M.gso; eauto. rewrite M.gss; eauto.
+  - edestruct (Hpre x') as [v1'' [Hget'' Hpre'']].
+    rewrite M.gso; eauto. rewrite M.gsspec in Hget.
+    destruct (Coqlib.peq x' y). inv Hget.
+    + eexists. rewrite M.gss; eauto. split; eauto.
+      eapply preord_val_refl.
+    + do 2 (rewrite M.gso in Hget''; eauto).
+      eexists. split; eauto.
+      do 2 (rewrite M.gso; eauto).
+Qed.
+
+Lemma def_funs_spec x v defs rho rho' :
+  M.get x (def_funs defs defs rho rho') = Some v ->
+  (name_in_fundefs x defs /\ v = cps.Vfun rho defs x) \/
+  (~ name_in_fundefs x defs /\ M.get x rho' = Some v).
+Proof.
+  generalize defs at 1 4. induction defs; intros defs' Hget.
+  - simpl in Hget. rewrite M.gsspec in Hget. destruct (Coqlib.peq x v0).
+    + inv Hget. left. split; eauto. constructor; eauto.
+    + edestruct (IHdefs _ Hget) as [[H1 H2] | [H1 H2]]; eauto.
+      * left. split; eauto. constructor 2; eauto.
+      * right. split; eauto. intros Hc. inv Hc; try congruence.
+  - simpl in Hget. right. split; eauto.
+Qed.
+
+Lemma def_funs_eq x defs rho rho' :
+  name_in_fundefs x defs ->
+  M.get x (def_funs defs defs rho rho') = Some (cps.Vfun rho defs x).
+Proof.
+  generalize defs at 2 4. induction defs; intros defs' Hin; inv Hin.
+  - simpl. rewrite M.gss. eauto.
+  - simpl. rewrite M.gsspec. destruct (Coqlib.peq x v); subst; eauto.
+Qed.
+
+Lemma def_funs_neq x defs rho rho' :
+  ~ name_in_fundefs x defs ->
+  M.get x (def_funs defs defs rho rho') = M.get x rho'.
+Proof.
+  generalize defs at 2. induction defs; intros defs' Hin; simpl; eauto.
+  rewrite M.gsspec. destruct (Coqlib.peq x v); subst; eauto.
+  exfalso. apply Hin. constructor; eauto. eapply IHdefs.
+  intros Hc.  eapply Hin. constructor 2; eauto.
+Qed.
+
+Require Import Omega.
+
+Lemma preord_env_def_funs_permut (k : nat) (f1 f2 : fundefs)
+      (rho1 rho2 : env) :
+  preord_env k rho1 rho2 ->
+  (forall f, name_in_fundefs f f1 -> ~ name_in_fundefs f f2) ->
+  preord_env k (def_funs f1 f1 rho1 (def_funs f2 f2 rho1 rho1))
+             (def_funs f2 f2 rho2 (def_funs f1 f1 rho2 rho2)).
+Proof.
+  intros Henv Hname x v Hget.
+  eapply def_funs_spec in Hget. destruct Hget as [[H1 H2] | [H1 H2]].
+  - eexists. rewrite def_funs_neq; eauto. rewrite def_funs_eq; eauto.
+    split; eauto. inv H2.
+    rewrite preord_val_eq. intros vs1 vs2 j t1 xs1 e1 rho1'' Hlen Hdef Heq.
+    edestruct (setlist_length (def_funs f1 f1 rho1 rho1)
+                              (def_funs f1 f1 rho2 rho2)) as [rho2'' Hset]; eauto.
+    do 4 eexists; repeat split; eauto. intros Hlt Hall.
+    eapply preord_exp_refl.
+    eapply preord_env_setlist_l. eapply preord_env_def_funs.
+    eapply preord_env_monotonic; [| eauto]. omega. eauto. eauto. eauto.
+  - eapply def_funs_spec in H2.
+    destruct H2 as [[H3 H4] | [H3 H4]]; subst.
+    + eexists. rewrite def_funs_eq; eauto. split; eauto.
+      rewrite preord_val_eq. intros vs1 vs2 j t1 xs1 e1 rho1' Hlen Hdef Heq.
+      edestruct (setlist_length (def_funs f2 f2 rho1 rho1)
+                                (def_funs f2 f2 rho2 rho2)) as [rho2' Hset]; eauto.
+      do 4 eexists; repeat split; eauto. intros Hlt Hall.
+      eapply preord_exp_refl.
+      eapply preord_env_setlist_l. eapply preord_env_def_funs.
+      eapply preord_env_monotonic; [| eauto]. omega. eauto. eauto. eauto.
+    + edestruct Henv as [v2 [Hget Hpre]]; eauto.
+      eexists. rewrite def_funs_neq; eauto. rewrite def_funs_neq; eauto.
+Qed.
+
+
+
+Lemma preord_env_def_funs_weaken (k : nat) (f1 f2 : fundefs)
+      (rho1 rho2 : env) :
+  (forall f, name_in_fundefs f f1 -> ~ name_in_fundefs f f2) ->
+  preord_env k (def_funs f1 f1 rho1 (def_funs f2 f2 rho1 rho1))
+             (def_funs f2 f2 rho2 (def_funs f1 f1 rho2 rho2)) ->
+  preord_env k (def_funs f1 f1 (def_funs f2 f2 rho1 rho1) (def_funs f2 f2 rho1 rho1))
+             (def_funs f2 f2 (def_funs f1 f1 rho2 rho2) (def_funs f1 f1 rho2 rho2)).
+Proof.
+  intros Henv Hname x v Hget. 
+  eapply def_funs_spec in Hget. destruct Hget as [[H1 H2] | [H1 H2]].
+  - eexists. rewrite def_funs_neq; eauto. rewrite def_funs_eq; eauto.
+    split; eauto. inv H2.
+    rewrite preord_val_eq. intros vs1 vs2 j t1 xs1 e1 rho1'' Hlen Hdef Heq.
+    edestruct (setlist_length (def_funs f1 f1 (def_funs f2 f2 rho1 rho1)
+                                        (def_funs f2 f2 rho1 rho1))
+                              (def_funs f1 f1 rho2 rho2)) as [rho2'' Hset]; eauto.
+    do 4 eexists; repeat split; eauto. intros Hlt Hall. admit.
+    (* eapply preord_exp_refl. *)
+    (* eapply preord_env_setlist_l. eapply preord_env_def_funs. *)
+    (* eapply preord_env_monotonic; [| eauto]. omega. eauto. eauto. eauto. *)
+  - eapply def_funs_spec in H2.
+    destruct H2 as [[H3 H4] | [H3 H4]]; subst.
+    + eexists. rewrite def_funs_eq; eauto. split; eauto.
+      rewrite preord_val_eq. intros vs1 vs2 j t1 xs1 e1 rho1' Hlen Hdef Heq.
+      edestruct (setlist_length (def_funs f2 f2 rho1 rho1)
+                                (def_funs f2 f2 (def_funs f1 f1 rho2 rho2)
+                                          (def_funs f1 f1 rho2 rho2))) as [rho2' Hset]; eauto.
+      do 4 eexists; repeat split; eauto. intros Hlt Hall.
+      eapply preord_exp_refl. 
+      eapply preord_env_setlist_l; eauto. eapply preord_env_def_funs.
+      eapply preord_env_monotonic; [| eauto]. omega. eauto. eauto. eauto.
+    + edestruct Henv as [v2 [Hget Hpre]]; eauto.
+      eexists. rewrite def_funs_neq; eauto. rewrite def_funs_neq; eauto.
+  Qed.
+
+        
+ *)   
