theories/L6_PCPS/set_util.v
@@ -1,0 +1,194 @@
+Require Import PArith Coq.MSets.MSetRBT Morphisms.
+
+Module PS := MSetRBT.Make POrderedType.Positive_as_OT.
+
+Import PS.
+
+Ltac inv H := inversion H; clear H; subst.
+
+(** Some set lemmas that might be useful *)
+Lemma Subset_add s s' e :
+  Subset s s' ->
+  Subset (add e s) (add e s').
+Proof.
+  intros H e' HIn. eapply add_spec in HIn.
+  inv HIn; eapply add_spec; eauto. 
+Qed.
+
+Lemma Subset_union_l s s' s'' :
+  Subset s s' ->
+  Subset (union s'' s) (union s'' s').
+Proof.
+  intros H e' HIn. eapply union_spec in HIn.
+  inv HIn; eapply union_spec; eauto. 
+Qed.
+
+Lemma Subset_union_r s s' s'' :
+  Subset s s' ->
+  Subset (union s s'') (union s' s'').
+Proof.
+  intros H e' HIn. eapply union_spec in HIn.
+  inv HIn; eapply union_spec; eauto. 
+Qed.
+
+Lemma Subset_refl s :
+  Subset s s.
+Proof.
+  intros H e; eauto. 
+Qed.
+
+Lemma Subset_union_mon_l s s' s'' :
+  Subset s s' ->
+  Subset s (union s' s'').
+Proof.
+  intros H e' HIn.
+  eapply union_spec; eauto. 
+Qed.
+
+Lemma Subset_union_mon_r s s' s'' :
+  Subset s s' ->
+  Subset s (union s'' s').
+Proof.
+  intros H e' HIn.
+  eapply union_spec; eauto. 
+Qed.
+
+Definition union_list (s : PS.t) (l : list elt) : PS.t :=
+  List.fold_left (fun set e => add e set) l s.
+
+Lemma union_list_spec (s : PS.t) (l : list elt) : 
+  forall (x : elt), In x (union_list s l) <->
+                    In x s \/ List.In x l.
+Proof.
+  revert s; induction l as [| x xs IHxs ]; simpl;
+  intros s e; split; intros H; eauto.
+  - inv H; eauto. contradiction.
+  - eapply IHxs in H. inversion H as [H1 | H2]; eauto.
+    eapply add_spec in H1; inv H1; eauto.
+  - inversion H as [H1 | [ H2 | H3 ]]; subst;
+    eapply IHxs; solve [ left; eapply add_spec; eauto
+                       | right; eauto ].
+Qed.
+
+Definition diff_list (s : PS.t) (l : list elt) : PS.t :=
+  List.fold_left (fun set e => remove e set) l s.
+
+Lemma diff_list_spec (s : PS.t) (l : list elt) : 
+  forall (x : elt), In x (diff_list s l) <->
+                    In x s /\ ~ List.In x l.
+Proof.
+  revert s; induction l as [| x xs IHxs ]; simpl;
+  intros s e; split; intros H; eauto.
+  - inv H; eauto.
+  - eapply IHxs in H. inversion H as [H1 H2]; eauto.
+    eapply remove_spec in H1; inv H1; split; eauto.
+    intros [Hc | Hc]; congruence.
+  - eapply IHxs. inversion H as [H1 H2]. split.
+    * eapply remove_spec. split; eauto.
+    * intros Hc. eauto.
+Qed.
+
+
+Lemma Subset_union_list s s' l :
+  Subset s s' ->
+  Subset (union_list s l) (union_list s' l).
+Proof.
+  intros H e' HIn. eapply union_list_spec in HIn.
+  inv HIn; eapply union_list_spec; eauto. 
+Qed.
+
+Lemma eq_lists (l1 l2 : list elt) :
+  Sorted.Sorted (fun x y : positive => (x ?= y)%positive = Lt) l1 ->
+  Sorted.Sorted (fun x y : positive => (x ?= y)%positive = Lt) l2 ->
+  SetoidList.NoDupA Logic.eq l1 ->
+  SetoidList.NoDupA Logic.eq l2 ->
+  (forall x, SetoidList.InA Logic.eq x l1 <-> SetoidList.InA Logic.eq x l2) ->
+  l1 = l2.
+Proof.
+  revert l2. induction l1; intros l2  Hs1 Hs2 Hd1 Hd2 Helem.
+  - destruct l2; eauto.
+    exfalso. specialize (Helem e).
+    assert (Hc : SetoidList.InA Logic.eq e nil)
+      by (eapply Helem; constructor; eauto).
+    inv Hc.
+  - destruct l2; eauto.
+    + exfalso. specialize (Helem a).
+      assert (Hc : SetoidList.InA Logic.eq a nil)
+        by (eapply Helem; constructor; eauto).
+      inv Hc.
+    + inv Hs1. inv Hs2. inv Hd1. inv Hd2.
+      assert (Helem' :
+                forall x, SetoidList.InA Logic.eq x l1 <->
+                          SetoidList.InA Logic.eq x l2).
+      { intros x. split; intros H. 
+        - assert (HIn : SetoidList.InA Logic.eq x (e :: l2))
+            by (eapply Helem; constructor 2; eauto).
+          inv HIn; eauto.
+          assert (HIn' : SetoidList.InA Logic.eq a (e :: l2))
+            by (eapply Helem; constructor; eauto).
+          assert (Hlt : (a ?= e)%positive = Lt).
+          { eapply SetoidList.SortA_InfA_InA
+            with (ltA := fun x y : positive => (x ?= y)%positive = Lt).
+            apply eq_equivalence. eapply E.lt_strorder.
+            apply E.lt_compat.
+            apply H1. eauto. eauto. }
+          inv HIn'. exfalso. eapply E.lt_strorder; eauto.
+          assert (Hlt' : (e ?= a)%positive = Lt).
+          { eapply SetoidList.SortA_InfA_InA
+            with (ltA := fun x y : positive => (x ?= y)%positive = Lt).
+            apply eq_equivalence. eapply E.lt_strorder.
+            apply E.lt_compat.
+            apply H3. eauto. eauto. }
+          rewrite (@PositiveOrder.le_antisym e a); eauto; congruence.
+        - assert (HIn : SetoidList.InA Logic.eq x (a :: l1))
+            by (eapply Helem; constructor 2; eauto).
+          inv HIn; eauto.
+          assert (HIn' : SetoidList.InA Logic.eq e (a :: l1))
+            by (eapply Helem; constructor; eauto).
+          assert (Hlt : (e ?= a)%positive = Lt).
+          { eapply SetoidList.SortA_InfA_InA
+            with (ltA := fun x y : positive => (x ?= y)%positive = Lt).
+            apply eq_equivalence. eapply E.lt_strorder.
+            apply E.lt_compat.
+            apply H3. eauto. eauto. }
+          inv HIn'. exfalso. eapply E.lt_strorder; eauto.
+          assert (Hlt' : (a ?= e)%positive = Lt).
+          { eapply SetoidList.SortA_InfA_InA
+            with (ltA := fun x y : positive => (x ?= y)%positive = Lt).
+            apply eq_equivalence. eapply E.lt_strorder.
+            apply E.lt_compat.
+            apply H1. eauto. eauto. }
+          rewrite (@PositiveOrder.le_antisym a e); eauto; congruence. }
+      f_equal; eauto.  
+      assert (HIn' : SetoidList.InA Logic.eq e (a :: l1)) by
+          (eapply Helem; constructor; eauto).
+      assert (HIn : SetoidList.InA Logic.eq a (e :: l2)) by
+          (eapply Helem; constructor; eauto).
+      inv HIn'; try now apply Heq. inv HIn; eauto.
+      assert (Hlt : (a ?= e)%positive = Lt).
+      { eapply SetoidList.SortA_InfA_InA
+        with (ltA := fun x y : positive => (x ?= y)%positive = Lt).
+        apply eq_equivalence. eapply E.lt_strorder.
+        apply E.lt_compat.
+        apply H1. eauto. eauto. }
+      inv HIn; eauto.
+      assert (Hlt' : (e ?= a)%positive = Lt).
+      { eapply SetoidList.SortA_InfA_InA
+        with (ltA := fun x y : positive => (x ?= y)%positive = Lt).
+        apply eq_equivalence. eapply E.lt_strorder.
+        apply E.lt_compat.
+        apply H3. eauto. eauto. }
+      rewrite (@PositiveOrder.le_antisym a e); eauto; congruence.
+Qed.
+
+Lemma elements_eq s1 s2 :
+  eq s1 s2 ->
+  elements s1 = elements s2.
+Proof.
+  intros H. apply eq_lists.
+  apply elements_spec2. apply elements_spec2.
+  apply elements_spec2w. apply elements_spec2w.
+  intros x'; split; intros H';
+  eapply elements_spec1; eapply elements_spec1 in H';
+  eapply H; eauto.
+Qed.
